finished LowLevelEvm, which will be renamed to EvmOpcodes and then used to create an EVM-only bytecode interpreter for testing purposes

EvmTests/translate_test.rb
@@ -1,6 +1,6 @@
 require 'json'
 
-lllc_file = '~/winhome/Code/solidity/build/lllc/lllc'
+lllc_file = '/mnt/c/Users/yorix/winhome/Code/solidity/build/lllc/lllc'
 
 if ARGV.length < 1 then
   abort("Requires an argument (JSON file to translate)")
@@ -9,7 +9,7 @@ end
 name_j = ARGV[0]
 name_t = name_j.gsub ".json", ".thy"
 name_l = name_j.gsub ".json", ".lll"
-name_b = name_j.gsup ".json", ".bin"
+name_b = name_j.gsub ".json", ".out"
 
 f_json = File.open(name_j, "r")
 obj = JSON.load f_json
@@ -22,15 +22,44 @@ File.open(name_l, "w") { |f|
   f.write lll_code
 }
 
-system(lllc_file, name_l, :out => [name_b, "w"])
+system(lllc_file, name_l, "-x", :out => [name_b, "w"])
 
 f_b = File.open(name_b, "r")
 
 bin_code = f_b.read
 
+
 f_thy = File.open(name_t, "w")
 
+=begin
 
+env:
+- currentCoinbase, 
+- currentDifficulty
+- currentGasLimit
+- currentNumber
+- currentTimestamp
+- previousHash
+
+exec:
+-address, caller, data, gas, gasPrice, origin, value
+
+pre:
+- account (the hash)
+  - balance
+  - code
+  - nonce
+  - storage
+
+expect: (this is the key part)
+- account (the hash)
+  - storage
+    - mapping from keys to values
+      (special case "0x => 0")
+
+storage seems to be the only expect...
+
+=end
 
 
 # File.open(name_j, "r") do |f_json|
