EVM/Templates/README.md
@@ -1,0 +1,1 @@
+This directory contains some velocity templates used to generate LowLevelEvm.thy
